examples/miniML/compiler/bytecode/bytecodeTerminationScript.sml
@@ -1,13 +1,8 @@
 open HolKernel boolLib bossLib BytecodeTheory
 val _ = new_theory"bytecodeTermination"
 
-val (bc_fetch_aux_def, bc_fetch_aux_ind) =
-  Defn.tprove_no_defn ((bc_fetch_aux_def, bc_fetch_aux_ind),
-  WF_REL_TAC `measure (LENGTH o FST)` THEN SRW_TAC [] []);
 val _ = save_thm ("bc_fetch_aux_def", bc_fetch_aux_def);
-val _ = save_thm ("bc_fetch_aux_ind", bc_fetch_aux_ind);
 val _ = export_rewrites["bc_fetch_aux_def"];
-
 val _ = save_thm("bc_fetch_def",bc_fetch_def);
 val _ = save_thm("bump_pc_def",bump_pc_def);
 val _ = save_thm("bc_find_loc_def",bc_find_loc_def);
@@ -16,6 +11,7 @@ val _ = save_thm("bc_next_ind",bc_next_ind);
 val _ = save_thm("bc_next_cases",bc_next_cases);
 val _ = save_thm("bc_stack_op_cases",bc_stack_op_cases);
 val _ = save_thm("bool_to_int_def",bool_to_int_def);
-val _ = save_thm("calc_len_def",calc_len_def);
+val _ = save_thm("is_Label_def",is_Label_def);
+val _ = export_rewrites["is_Label_def"];
 
 val _ = export_theory()
